prop: modeling relation

type-theory-IMC010/prop.v
@@ -6,6 +6,7 @@
 *)
 
 Require Import Coq.Lists.List.
+Require Import Coq.Arith.EqNat.
 
 Inductive form : Set :=
  | f_var : nat -> form
@@ -63,3 +64,59 @@ Example findvars_all :
  find_variables (f_and (f_or (f_neg (f_var 1)) (f_var 2)) (f_imp (f_var 3) (f_var 4)))
   = 4 :: 3 :: 2 :: 1 :: nil.
 Proof. reflexivity. Qed.
+
+
+(* Checks whether the given number x is in the list l *)
+Definition bin_nat (x:nat) (l:list nat) : bool :=
+ existsb (fun y => beq_nat x y) l.
+
+
+(* Given a model and a formula f, checks whether the model satisfies the formula.
+
+   read: m |= f
+*)
+Fixpoint models (m:model) (f:form) {struct f} : bool :=
+ match f with
+ | f_var x   => bin_nat x m
+ | f_and l r => andb  (models m l) (models m r)
+ | f_or  l r => orb   (models m l) (models m r)
+ | f_imp l r => implb (models m l) (models m r)
+ | f_neg g   => negb  (models m g)
+ end
+ .
+
+Example models_var :
+ models (1::nil) (f_var 1) = true.
+Proof. simpl. reflexivity. Qed.
+
+Example models_and :
+ models (1::2::nil) (f_and (f_var 2) (f_var 1)) = true.
+Proof. simpl. reflexivity. Qed.
+
+Example not_models_and :
+ models (1::nil) (f_and (f_var 2) (f_var 1)) = false.
+Proof. simpl. reflexivity. Qed.
+
+Example model_or :
+ models (1::nil) (f_or (f_var 42) (f_var 1)) = true.
+Proof. simpl. reflexivity. Qed.
+
+Example not_models_or :
+ models (1::2::nil) (f_or (f_var 42) (f_var 43)) = false.
+Proof. simpl. reflexivity. Qed.
+
+Example models_imp :
+ models nil (f_imp (f_var 1) (f_var 1)) = true.
+Proof. simpl. reflexivity. Qed.
+
+Example not_models_imp :
+ models (1::nil) (f_imp (f_var 1) (f_var 42)) = false.
+Proof. simpl. reflexivity. Qed.
+
+Example models_neg :
+ models nil (f_neg (f_var 42)) = true.
+Proof. simpl. reflexivity. Qed.
+
+Example not_models_neg :
+ models (1::nil) (f_neg (f_var 1)) = false.
+Proof. simpl. reflexivity. Qed.
